formal/inference/heuristics/Store_Reuse_Subsumption.thy
@@ -513,10 +513,12 @@ lemma generalise_output_directly_subsumes_original_executable:
      apply simp+
   by (simp add: generalise_output_context_check_def generalise_output_directly_subsumes_original)
 
+(* t' is the generalised transition *)
 primrec input_i_stored_in_reg :: "transition \<Rightarrow> transition \<Rightarrow> nat \<Rightarrow> nat \<Rightarrow> (nat \<times> nat) option" where
   "input_i_stored_in_reg t' t i 0 = (if is_generalisation_of t' t i 0 then Some (i, 0) else None)" |
   "input_i_stored_in_reg t' t i (Suc r) = (if is_generalisation_of t' t i (Suc r) then Some (i, (Suc r)) else input_i_stored_in_reg t' t i r)"
 
+(* t' is the generalised transition *)
 primrec input_stored_in_reg_aux :: "transition \<Rightarrow> transition \<Rightarrow> nat \<Rightarrow> nat \<Rightarrow> (nat \<times> nat) option" where
   "input_stored_in_reg_aux t' t 0 r = input_i_stored_in_reg t' t 0 r" |
   "input_stored_in_reg_aux t' t (Suc i) r = (case input_i_stored_in_reg t' t (Suc i) r of
@@ -524,8 +526,12 @@ primrec input_stored_in_reg_aux :: "transition \<Rightarrow> transition \<Righta
                                               Some (i, r) \<Rightarrow> Some (i, r)
                                             ) "
 
+(* t' is the generalised transition *)
 definition input_stored_in_reg :: "transition \<Rightarrow> transition \<Rightarrow> iEFSM \<Rightarrow> (nat \<times> nat) option" where
-  "input_stored_in_reg t' t e = input_stored_in_reg_aux t' t (max_reg e) (max_input e)"
+  "input_stored_in_reg t' t e = (case input_stored_in_reg_aux t' t (max_reg e) (max_input e) of
+                                 None \<Rightarrow> None |
+                                 Some (i, r) \<Rightarrow> if length (filter (\<lambda>(r', u). r' = R r) (Updates t')) = 1 then Some (i, r) else None
+)"
 
 definition initially_undefined_context_check :: "iEFSM \<Rightarrow> nat \<Rightarrow> nat \<Rightarrow> bool" where
   "initially_undefined_context_check e r s = (\<forall>t. accepts_trace (tm e) t \<and> gets_us_to s (tm e) 0 <>  t \<longrightarrow> (anterior_context (tm e) t) (V (R r)) = {|Undef|} \<and> (\<forall>i. (anterior_context (tm e) t) (V (I i)) = {|Bc True|}))"
@@ -575,7 +581,14 @@ qed
 
 
 lemma input_stored_in_reg_aux_is_generalisation: "input_stored_in_reg t' t e = Some (i, r) \<Longrightarrow> is_generalisation_of t' t i r"
-  by (simp add: input_stored_in_reg_def input_stored_in_reg_aux_is_generalisation_aux)
+  apply (simp add: input_stored_in_reg_def)
+  apply (cases "input_stored_in_reg_aux t' t (max_reg e) (max_input e)")
+   apply simp
+  apply (case_tac a)
+  apply simp
+  apply (case_tac "length (filter (\<lambda>(r', u). r' = R b) (Updates t')) = 1")
+   apply (simp add: input_stored_in_reg_aux_is_generalisation_aux)
+  by simp
 
 (*
   This allows us to call these three functions for direct subsumption of generalised
@@ -603,7 +616,8 @@ definition drop_guard_add_update_direct_subsumption :: "transition \<Rightarrow>
   "drop_guard_add_update_direct_subsumption t' t e s' = (case input_stored_in_reg t' t e of None \<Rightarrow> False |
    Some (i, r) \<Rightarrow> if no_illegal_updates t r then initially_undefined_context_check e r s' else False)"
 
-lemma drop_guard_add_update_direct_subsumption_implies_direct_subsumption: "drop_guard_add_update_direct_subsumption t' t e s' \<Longrightarrow> directly_subsumes e1 e s s' t' t"
+lemma drop_guard_add_update_direct_subsumption_implies_direct_subsumption:
+  "drop_guard_add_update_direct_subsumption t' t e s' \<Longrightarrow> directly_subsumes e1 e s s' t' t"
   apply (simp add: drop_guard_add_update_direct_subsumption_def)
   apply (case_tac "input_stored_in_reg t' t e")
    apply simp+
@@ -613,4 +627,122 @@ lemma drop_guard_add_update_direct_subsumption_implies_direct_subsumption: "drop
    apply (simp add: generalised_directly_subsumes_original)
   by simp
 
+lemma input_stored_in_reg_in_updates: "input_stored_in_reg t t' e = Some (aa, ba) \<Longrightarrow> (R ba, V (I aa)) \<in> set (Updates t)"
+proof(induction "Updates t")
+  case Nil
+  then show ?case
+    using input_stored_in_reg_def Nil.prems generalised_updates input_stored_in_reg_aux_is_generalisation by fastforce
+next
+  case (Cons a x)
+  then show ?case
+    using input_stored_in_reg_def Cons.prems generalised_updates input_stored_in_reg_aux_is_generalisation by fastforce
+qed
+
+lemma input_stored_in_reg_reg_updated_once: "input_stored_in_reg t t' e = Some (aa, r) \<Longrightarrow>
+       length (filter (\<lambda>(r', u). r' = R r) (Updates t)) = 1"
+  apply (simp add: input_stored_in_reg_def)
+  apply (case_tac "input_stored_in_reg_aux t t' (max_reg e) (max_input e)")
+   apply simp
+  apply (case_tac a)
+  apply clarify
+  apply simp
+  apply (case_tac "length (filter (\<lambda>(r', u). r' = R ba) (Updates t)) = 1")
+  by auto
+
+lemma only_one_update: "length (filter (\<lambda>(r', u). r' = R r) U) = 1 \<Longrightarrow>
+      (R r, V (I aa)) \<in> set U \<Longrightarrow>
+      (R r, u) \<in> set U \<Longrightarrow>
+       u = V (I aa)"
+proof(induct U)
+  case Nil
+  then show ?case by simp
+next
+  case (Cons a U)
+  then show ?case
+    apply simp
+    apply (case_tac a)
+    apply simp
+    apply clarify
+    apply (case_tac "ab = R r")
+     apply simp
+     apply (metis (mono_tags, lifting) case_prod_conv filter_empty_conv)
+    by simp
+qed
+
+lemma register_updated_once:
+  "input_stored_in_reg t t' e = Some (aa, ba) \<Longrightarrow>
+  \<forall>u. (R ba, u) \<in> set (Updates t) \<longrightarrow> u = V (I aa)"
+  using only_one_update input_stored_in_reg_reg_updated_once input_stored_in_reg_in_updates by blast
+
+lemma remove_obsolete_constraints_leaves_registers: 
+       "remove_obsolete_constraints (Contexts.apply_updates (medial c (Guard t)) c (Updates t)) (fst |`| fset_of_list (Updates t)) (V (R r)) =
+       (Contexts.apply_updates (medial c (Guard t)) c (Updates t)) (V (R r))"
+  apply (simp add: remove_obsolete_constraints_def no_illegal_updates_def)
+  by auto
+
+lemma input_stored_in_reg_aux_not_none: "input_stored_in_reg t t' e = Some (aa, ba) \<Longrightarrow>
+input_stored_in_reg_aux t t' (max_reg e) (max_input e) \<noteq> None"
+  apply (simp add: input_stored_in_reg_def)
+  apply (cases "input_stored_in_reg_aux t t' (max_reg e) (max_input e)")
+  by auto
+
+lemma input_stored_in_reg_updatess_reg_to_input: 
+      "input_stored_in_reg t t' e = Some (aa, ba) \<Longrightarrow>
+       consistent (medial c (Guard t)) \<Longrightarrow>
+       posterior c t (V (R ba)) = (medial c (Guard t)) (V (I aa))"
+  apply (simp add: posterior_def posterior_separate_def)
+  apply (simp add: remove_obsolete_constraints_leaves_registers)
+  using generalised_updates input_stored_in_reg_aux_is_generalisation by fastforce
+
+lemma input_stored_in_reg_guards_input: "input_stored_in_reg t t' e = Some (aa, ba) \<Longrightarrow> (\<exists> v. gexp.Eq (V (I aa)) (L v) \<in> set (Guard t'))"
+  apply (simp add: input_stored_in_reg_def)
+  apply (case_tac "input_stored_in_reg_aux t t' (max_reg e) (max_input e)")
+   apply simp
+  apply simp
+  apply (case_tac a)
+  apply clarify
+  apply simp
+  apply (case_tac "length (filter (\<lambda>(r', u). r' = R baa) (Updates t)) = 1")
+   defer
+   apply simp
+  apply simp
+  apply clarify
+  apply simp
+  apply (case_tac "max_reg e")
+   apply (case_tac "max_input e")
+    apply simp
+    apply (case_tac "is_generalisation_of t t' 0 0")
+     apply (simp add: is_generalisation_of_def)
+    apply simp
+   apply (case_tac "is_generalisation_of t t' 0 (Suc nat)")
+    apply (simp add: is_generalisation_of_def)
+  using input_stored_in_reg_aux_is_generalisation_aux is_generalisation_of_def apply blast
+  apply simp
+  apply (case_tac "max_input e")
+   apply simp
+   apply (case_tac "is_generalisation_of t t' (Suc nat) 0")
+    apply (simp add: is_generalisation_of_def)
+   apply simp
+   apply (metis fst_conv is_generalisation_of_def option.inject option.simps(3))
+  apply simp
+  apply (case_tac "is_generalisation_of t t' (Suc nat) (Suc nata)")
+   apply (simp add: is_generalisation_of_def)
+  apply simp
+  by (metis (no_types, lifting) input_i_stored_in_reg.simps(2) input_stored_in_reg_aux.simps(2) input_stored_in_reg_aux_is_generalisation_aux is_generalisation_of_def)
+
+lemma input_stored_in_reg_medial_not_undef:
+  "input_stored_in_reg t t' e = Some (aa, ba) \<Longrightarrow>
+   medial c (Guard t') (V (I aa)) \<noteq> {|Undef|}"
+  using input_stored_in_reg_guards_input[of t t' e aa ba]
+  using equality_guard_gives_equality_constraint[of aa "Guard t'" c]
+  by auto
+
+lemma input_stored_in_reg_medial_equiv: "input_stored_in_reg t t' e = Some (aa, ba) \<Longrightarrow>
+       medial c (Guard t @ Guard t') = medial c (Guard t')"
+  using input_stored_in_reg_aux_is_generalisation[of t t' e aa ba]
+  apply simp
+  using generalisation_medial_equiv[of t t' aa ba c]
+  apply simp
+  using medial_append_commutative
+  by simp
 end
